To solve the given problem, let's break it into steps. The problem asks to evaluate the line integral ∫CF⋅dr\int_C \mathbf{F} \cdot d\mathbf{r} where:

- F=zi+xj+yk\mathbf{F} = z\mathbf{i} + x\mathbf{j} + y\mathbf{k},
- The curve CC is parametrized as r(t)=cos⁡ti+sin⁡tj+tk\mathbf{r}(t) = \cos t \mathbf{i} + \sin t \mathbf{j} + t \mathbf{k} for t∈[0,2π]t \in [0, 2\pi].

### Step 1: Find drd\mathbf{r}

The differential drd\mathbf{r} is the derivative of r(t)\mathbf{r}(t) with respect to tt, multiplied by dtdt:

r(t)=cos⁡ti+sin⁡tj+tk,\mathbf{r}(t) = \cos t \mathbf{i} + \sin t \mathbf{j} + t \mathbf{k}, drdt=−sin⁡ti+cos⁡tj+k,\frac{d\mathbf{r}}{dt} = -\sin t \mathbf{i} + \cos t \mathbf{j} + \mathbf{k}, dr=(−sin⁡ti+cos⁡tj+k)dt.d\mathbf{r} = (-\sin t \mathbf{i} + \cos t \mathbf{j} + \mathbf{k}) dt.

### Step 2: Express F\mathbf{F} in terms of tt

From the curve r(t)\mathbf{r}(t), we know:

x=cos⁡t,y=sin⁡t,z=t.x = \cos t, \quad y = \sin t, \quad z = t.

Substituting into F=zi+xj+yk\mathbf{F} = z\mathbf{i} + x\mathbf{j} + y\mathbf{k}:

F=ti+cos⁡tj+sin⁡tk.\mathbf{F} = t \mathbf{i} + \cos t \mathbf{j} + \sin t \mathbf{k}.

### Step 3: Compute F⋅dr\mathbf{F} \cdot d\mathbf{r}

The dot product F⋅dr\mathbf{F} \cdot d\mathbf{r} is:

F⋅dr=(ti+cos⁡tj+sin⁡tk)⋅(−sin⁡ti+cos⁡tj+k)dt.\mathbf{F} \cdot d\mathbf{r} = (t \mathbf{i} + \cos t \mathbf{j} + \sin t \mathbf{k}) \cdot (-\sin t \mathbf{i} + \cos t \mathbf{j} + \mathbf{k}) dt.

Performing the dot product:

F⋅dr=t(−sin⁡t)+cos⁡t(cos⁡t)+sin⁡t(1) dt,\mathbf{F} \cdot d\mathbf{r} = t(-\sin t) + \cos t(\cos t) + \sin t(1) \, dt, F⋅dr=−tsin⁡t+cos⁡2t+sin⁡t dt.\mathbf{F} \cdot d\mathbf{r} = -t \sin t + \cos^2 t + \sin t \, dt.

### Step 4: Simplify and integrate

The integral becomes:

∫CF⋅dr=∫02π(−tsin⁡t+cos⁡2t+sin⁡t)dt.\int_C \mathbf{F} \cdot d\mathbf{r} = \int_0^{2\pi} \left(-t \sin t + \cos^2 t + \sin t \right) dt.

Split into three terms:

∫02πF⋅dr=∫02π(−tsin⁡t)dt+∫02πcos⁡2t dt+∫02πsin⁡t dt.\int_0^{2\pi} \mathbf{F} \cdot d\mathbf{r} = \int_0^{2\pi} (-t \sin t) dt + \int_0^{2\pi} \cos^2 t \, dt + \int_0^{2\pi} \sin t \, dt.

1. **First term**: ∫02π−tsin⁡t dt\int_0^{2\pi} -t \sin t \, dt: Use integration by parts: u=t, dv=sin⁡tdtu = t, \, dv = \sin t dt. Then, du=dt, v=−cos⁡tdu = dt, \, v = -\cos t:
    
    ∫tsin⁡tdt=−tcos⁡t+∫cos⁡tdt=−tcos⁡t+sin⁡t.\int t \sin t dt = -t \cos t + \int \cos t dt = -t \cos t + \sin t.
    
    Evaluate from 00 to 2π2\pi:
    
    [−tcos⁡t+sin⁡t]02π=[−2πcos⁡(2π)+sin⁡(2π)]−[−0⋅cos⁡(0)+sin⁡(0)]=0.\left[-t \cos t + \sin t \right]_0^{2\pi} = \left[-2\pi \cos(2\pi) + \sin(2\pi)\right] - \left[-0 \cdot \cos(0) + \sin(0)\right] = 0.
2. **Second term**: ∫02πcos⁡2t dt\int_0^{2\pi} \cos^2 t \, dt: Use the identity cos⁡2t=1+cos⁡(2t)2\cos^2 t = \frac{1 + \cos(2t)}{2}:
    
    ∫02πcos⁡2tdt=∫02π12dt+∫02πcos⁡(2t)2dt.\int_0^{2\pi} \cos^2 t dt = \int_0^{2\pi} \frac{1}{2} dt + \int_0^{2\pi} \frac{\cos(2t)}{2} dt.
    
    The first term is:
    
    ∫02π12dt=12⋅2π=π.\int_0^{2\pi} \frac{1}{2} dt = \frac{1}{2} \cdot 2\pi = \pi.
    
    The second term is:
    
    ∫02πcos⁡(2t)2dt=0(since cosine over a full period is zero).\int_0^{2\pi} \frac{\cos(2t)}{2} dt = 0 \quad \text{(since cosine over a full period is zero)}.
    
    Thus, ∫02πcos⁡2tdt=π\int_0^{2\pi} \cos^2 t dt = \pi.
    
3. **Third term**: ∫02πsin⁡t dt\int_0^{2\pi} \sin t \, dt:
    
    ∫02πsin⁡tdt=[−cos⁡t]02π=−cos⁡(2π)+cos⁡(0)=0.\int_0^{2\pi} \sin t dt = \left[-\cos t \right]_0^{2\pi} = -\cos(2\pi) + \cos(0) = 0.

### Step 5: Combine results

∫CF⋅dr=0+π+0=π.\int_C \mathbf{F} \cdot d\mathbf{r} = 0 + \pi + 0 = \pi.

Thus, the given statement holds, and the result is:

3π.\boxed{3\pi}.